restored the old code

Given_Clause_Loops/Prover_Lazy_List_Queue.thy
@@ -13,214 +13,576 @@ theory Prover_Lazy_List_Queue
 begin
 
 
+subsection \<open>Basic Lemmas\<close>
+
+lemma ne_and_in_set_take_imp_in_set_take_remove:
+  assumes
+    "z \<noteq> y" and
+    "z \<in> set (take m xs)"
+  shows "z \<in> set (take m (remove1 y xs))"
+  using assms
+proof (induct xs arbitrary: m)
+  case (Cons x xs)
+  note ih = this(1) and z_ne_y = this(2) and z_in_take_xxs = this(3)
+
+  show ?case
+  proof (cases "z = x")
+    case True
+    thus ?thesis
+      by (metis (no_types, lifting) List.hd_in_set gr_zeroI hd_take in_set_remove1 list.sel(1)
+          remove1.simps(2) take_eq_Nil z_in_take_xxs z_ne_y)
+  next
+    case z_ne_x: False
+
+    have z_in_take_xs: "z \<in> set (take m xs)"
+      using z_in_take_xxs z_ne_x
+      by (smt (verit, del_insts) butlast_take in_set_butlastD in_set_takeD le_cases3 set_ConsD
+          take_Cons' take_all)
+
+    show ?thesis
+    proof (cases "y = x")
+      case y_eq_x: True
+      show ?thesis
+        using y_eq_x by (simp add: z_in_take_xs)
+    next
+      case y_ne_x: False
+
+      have "m > 0"
+        by (metis gr0I list.set_cases list.simps(3) take_Cons' z_in_take_xxs)
+      then obtain m' :: nat where
+        m: "m = Suc m'"
+        using gr0_implies_Suc by presburger
+
+      have z_in_take_xs': "z \<in> set (take m' xs)"
+        using z_in_take_xs z_in_take_xxs z_ne_x by (simp add: m)
+      note ih = ih[OF z_ne_y z_in_take_xs']
+
+      show ?thesis
+        using y_ne_x ih unfolding m by simp
+    qed
+  qed
+qed simp
+
+lemma in_set_take_imp_in_set_take_fold_append_single:
+  assumes "x \<in> set (take n xs)"
+  shows "x \<in> set (take n (fold (\<lambda>y ys. ys @ [y]) ys xs))"
+  using assms by (induct ys arbitrary: xs) auto
+
+lemma notin_set_and_in_set_take_imp_in_set_take_fold_remove1:
+  assumes
+    "x \<notin> set ys" and
+    "x \<in> set (take m xs)"
+  shows "x \<in> set (take m (fold remove1 ys xs))"
+  using assms
+proof (induct ys arbitrary: xs)
+  case (Cons y ys xs)
+  note ih = this(1) and x_ni_yys = this(2) and x_in_take_xs = this(3)
+
+  have x_ne_y: "x \<noteq> y"
+    using x_ni_yys by simp
+
+  have x_ni_ys: "x \<notin> set ys"
+    using x_ni_yys by simp
+  have x_in_take_rem_y_xs: "x \<in> set (take m (remove1 y xs))"
+    using x_in_take_xs x_ne_y using ne_and_in_set_take_imp_in_set_take_remove by fast
+  note ih = ih[OF x_ni_ys x_in_take_rem_y_xs]
+
+  show ?case
+    using ih by simp
+qed simp
+
+
 subsection \<open>Locales\<close>
 
 locale prover_lazy_list_queue =
   fixes
-    nil :: 's and
-    llist :: "'s \<Rightarrow> 'e llist" and
     empty :: 'q and
-    add_stream :: "'s \<Rightarrow> 'q \<Rightarrow> 'q" and
-    remove_stream :: "'s \<Rightarrow> 'q \<Rightarrow> 'q" and
+    add_llist :: "'e llist \<Rightarrow> 'q \<Rightarrow> 'q" and
+    remove_llist :: "'e llist \<Rightarrow> 'q \<Rightarrow> 'q" and
     pick_elem :: "'q \<Rightarrow> 'e \<times> 'q" and
-    streams :: "'q \<Rightarrow> 's multiset"
+    llists :: "'q \<Rightarrow> 'e llist multiset"
   assumes
-    llist_nil[simp]: "llist nil = LNil" and
-    exists_stream: "\<exists>s. llist s = xs" and
-    streams_empty[simp]: "streams empty = {#}" and
-    streams_not_empty: "Q \<noteq> empty \<Longrightarrow> streams Q \<noteq> {#}" and
-    streams_add[simp]: "streams (add_stream es Q) = streams Q + {#es#}" and
-    streams_remove[simp]: "streams (remove_stream es Q) = streams Q - {#es#}" and
-    streams_pick_elem: "(\<exists>s \<in># streams Q. llist s \<noteq> LNil) \<Longrightarrow>
-      \<exists>s \<in># streams Q. \<exists>s'. llist s \<noteq> LNil \<and> llist s' = ltl (llist s)
-        \<and> fst (pick_elem Q) = lhd (llist s)
-        \<and> streams (snd (pick_elem Q)) = streams Q - {#s#} + {#s'#}"
+    llists_empty[simp]: "llists empty = {#}" and
+    llists_not_empty: "Q \<noteq> empty \<Longrightarrow> llists Q \<noteq> {#}" and
+    llists_add[simp]: "llists (add_llist es Q) = llists Q + {#es#}" and
+    llist_remove[simp]: "llists (remove_llist es Q) = llists Q - {#es#}" and
+    llists_pick_elem: "(\<exists>es \<in># llists Q. es \<noteq> LNil) \<Longrightarrow>
+      \<exists>e es. LCons e es \<in># llists Q \<and> fst (pick_elem Q) = e
+        \<and> llists (snd (pick_elem Q)) = llists Q - {#LCons e es#} + {#es#}"
 begin
 
 abbreviation has_elem :: "'q \<Rightarrow> bool" where
-  "has_elem Q \<equiv> \<exists>s \<in># streams Q. llist s \<noteq> LNil"
+  "has_elem Q \<equiv> \<exists>es \<in># llists Q. es \<noteq> LNil"
 
 inductive lqueue_step :: "'q \<times> 'e set \<Rightarrow> 'q \<times> 'e set \<Rightarrow> bool" where
-  lqueue_step_fold_add_streamI:
-  "lqueue_step (Q, D) (fold add_stream ss Q, D - \<Union> {lset (llist s) |s. s \<in> set ss})"
-| lqueue_step_fold_remove_streamI:
-  "lqueue_step (Q, D) (fold remove_stream ss Q, D \<union> \<Union> {lset (llist s) |s. s \<in> set ss})"
+  lqueue_step_fold_add_llistI:
+  "lqueue_step (Q, D) (fold add_llist ess Q, D - \<Union> {lset es |es. es \<in> set ess})"
+| lqueue_step_fold_remove_llistI:
+  "lqueue_step (Q, D) (fold remove_llist ess Q, D \<union> \<Union> {lset es |es. es \<in> set ess})"
 | lqueue_step_pick_elemI: "has_elem Q \<Longrightarrow>
   lqueue_step (Q, D) (snd (pick_elem Q), D \<union> {fst (pick_elem Q)})"
 
 lemma lqueue_step_idleI: "lqueue_step QD QD"
-  using lqueue_step_fold_add_streamI[of "fst QD" "snd QD" "[]", simplified] .
+  using lqueue_step_fold_add_llistI[of "fst QD" "snd QD" "[]", simplified] .
 
-lemma lqueue_step_add_streamI: "lqueue_step (Q, D) (add_stream s Q, D - lset (llist s))"
-  using lqueue_step_fold_add_streamI[of _ _ "[s]", simplified] .
+lemma lqueue_step_add_llistI: "lqueue_step (Q, D) (add_llist es Q, D - lset es)"
+  using lqueue_step_fold_add_llistI[of _ _ "[es]", simplified] .
 
-lemma lqueue_step_remove_streamI: "lqueue_step (Q, D) (remove_stream s Q, D \<union> lset (llist s))"
-  using lqueue_step_fold_remove_streamI[of _ _ "[s]", simplified] .
+lemma lqueue_step_remove_llistI: "lqueue_step (Q, D) (remove_llist es Q, D \<union> lset es)"
+  using lqueue_step_fold_remove_llistI[of _ _ "[es]", simplified] .
 
-lemma streams_fold_add_stream[simp]: "streams (fold add_stream ss Q) = mset ss + streams Q"
-  by (induct ss arbitrary: Q) auto
+lemma llists_fold_add_llist[simp]: "llists (fold add_llist es Q) = mset es + llists Q"
+  by (induct es arbitrary: Q) auto
 
-lemma streams_fold_remove_stream[simp]: "streams (fold remove_stream ss Q) = streams Q - mset ss"
-  by (induct ss arbitrary: Q) auto
+lemma llists_fold_remove_llist[simp]: "llists (fold remove_llist es Q) = llists Q - mset es"
+  by (induct es arbitrary: Q) auto
 
-inductive
-  pick_lqueue_step_w_details :: "'q \<times> 'e set \<Rightarrow> 'e \<Rightarrow> 'e llist \<Rightarrow> 'q \<times> 'e set \<Rightarrow> bool"
-where
-  pick_lqueue_step_w_detailsI: "s \<in># streams Q \<Longrightarrow> llist s \<noteq> LNil \<Longrightarrow> llist s' = ltl (llist s) \<Longrightarrow>
-    fst (pick_elem Q) = lhd (llist s) \<Longrightarrow>
-    streams (snd (pick_elem Q)) = streams Q - {#s#} + {#s'#} \<Longrightarrow>
-    pick_lqueue_step_w_details (Q, D) (lhd (llist s)) (ltl (llist s))
-      (snd (pick_elem Q), D \<union> {lhd (llist s)})"
+inductive pick_lqueue_step_w_details :: "'q \<times> 'e set \<Rightarrow> 'e \<Rightarrow> 'e llist \<Rightarrow> 'q \<times> 'e set \<Rightarrow> bool" where
+  pick_lqueue_step_w_detailsI: "LCons e es \<in># llists Q \<Longrightarrow> fst (pick_elem Q) = e \<Longrightarrow>
+    llists (snd (pick_elem Q)) = llists Q - {#LCons e es#} + {#es#} \<Longrightarrow>
+    pick_lqueue_step_w_details (Q, D) e es (snd (pick_elem Q), D \<union> {e})"
 
 inductive pick_lqueue_step :: "'q \<times> 'e set \<Rightarrow> 'q \<times> 'e set \<Rightarrow> bool" where
   pick_lqueue_stepI: "pick_lqueue_step_w_details QD e es QD' \<Longrightarrow> pick_lqueue_step QD QD'"
 
-inductive remove_lqueue_step_w_details :: "'q \<times> 'e set \<Rightarrow> 's list \<Rightarrow> 'q \<times> 'e set \<Rightarrow> bool" where
+inductive
+  remove_lqueue_step_w_details :: "'q \<times> 'e set \<Rightarrow> 'e llist list \<Rightarrow> 'q \<times> 'e set \<Rightarrow> bool"
+where
   remove_lqueue_step_w_detailsI:
-    "remove_lqueue_step_w_details (Q, D) ss
-       (fold remove_stream ss Q, D \<union> \<Union> {lset (llist s) |s. s \<in> set ss})"
+    "remove_lqueue_step_w_details (Q, D) ess
+       (fold remove_llist ess Q, D \<union> \<Union> {lset es |es. es \<in> set ess})"
 
 end
 
 locale fair_prover_lazy_list_queue =
-  prover_lazy_list_queue nil llist empty add_stream remove_stream pick_elem streams
+  prover_lazy_list_queue empty add_llist remove_llist pick_elem llists
   for
-    nil :: 's and
-    llist :: "'s \<Rightarrow> 'e llist" and
     empty :: 'q and
-    add_stream :: "'s \<Rightarrow> 'q \<Rightarrow> 'q" and
-    remove_stream :: "'s \<Rightarrow> 'q \<Rightarrow> 'q" and
+    add_llist :: "'e llist \<Rightarrow> 'q \<Rightarrow> 'q" and
+    remove_llist :: "'e llist \<Rightarrow> 'q \<Rightarrow> 'q" and
     pick_elem :: "'q \<Rightarrow> 'e \<times> 'q" and
-    streams :: "'q \<Rightarrow> 's multiset" +
+    llists :: "'q \<Rightarrow> 'e llist multiset" +
   assumes fair: "chain lqueue_step QDs \<Longrightarrow> infinitely_often pick_lqueue_step QDs \<Longrightarrow>
-    s \<in># streams (fst (lnth QDs i)) \<Longrightarrow> llist s \<noteq> LNil \<Longrightarrow> llist s' = ltl (llist s) \<Longrightarrow>
-    \<exists>j \<ge> i. (\<exists>ss. s \<in> set ss \<and> remove_lqueue_step_w_details (lnth QDs j) ss (lnth QDs (Suc j)))
-      \<or> pick_lqueue_step_w_details (lnth QDs j) (lhd (llist s)) (ltl (llist s)) (lnth QDs (Suc j))"
+    LCons e es \<in># llists (fst (lnth QDs i)) \<Longrightarrow>
+    \<exists>j \<ge> i. (\<exists>ess. LCons e es \<in> set ess
+        \<and> remove_lqueue_step_w_details (lnth QDs j) ess (lnth QDs (Suc j)))
+      \<or> pick_lqueue_step_w_details (lnth QDs j) e es (lnth QDs (Suc j))"
 begin
 
 lemma fair_strong:
   assumes
     chain: "chain lqueue_step QDs" and
     inf: "infinitely_often pick_lqueue_step QDs" and
-    es_in: "s \<in># streams (fst (lnth QDs i))" and
-    k_lt: "enat k < llength (llist s)"
+    es_in: "es \<in># llists (fst (lnth QDs i))" and
+    k_lt: "enat k < llength es"
   shows "\<exists>j \<ge> i.
-    (\<exists>k' \<le> k. \<exists>ss. ldrop k' (llist s) \<in> set (map llist ss)
-       \<and> remove_lqueue_step_w_details (lnth QDs j) ss (lnth QDs (Suc j)))
-    \<or> pick_lqueue_step_w_details (lnth QDs j) (lnth (llist s) k) (ldrop (Suc k) (llist s))
-      (lnth QDs (Suc j))"
+    (\<exists>k' \<le> k. \<exists>ess. ldrop k' es \<in> set ess
+         \<and> remove_lqueue_step_w_details (lnth QDs j) ess (lnth QDs (Suc j)))
+       \<or> pick_lqueue_step_w_details (lnth QDs j) (lnth es k) (ldrop (Suc k) es) (lnth QDs (Suc j))"
   using k_lt
 proof (induct k)
   case 0
   note zero_lt = this
-
-  have nnil: "llist s \<noteq> LNil"
-    using zero_lt by force
-
-  obtain s' :: 's where
-    s': "llist s' = ltl (llist s)"
-    using exists_stream by blast
-
-  obtain j where
-    j_ge: "j \<ge> i" and
-    rem_or_pick:
-      "(\<exists>ss. s \<in> set ss \<and> remove_lqueue_step_w_details (lnth QDs j) ss (lnth QDs (Suc j)))
-       \<or> pick_lqueue_step_w_details (lnth QDs j) (lhd (llist s)) (ltl (llist s)) (lnth QDs (Suc j))"
-    using fair[OF chain inf es_in nnil s'] by blast
-
-  {
-    assume "\<exists>ss. s \<in> set ss \<and> remove_lqueue_step_w_details (lnth QDs j) ss (lnth QDs (Suc j))"
-    hence "\<exists>ss. ldrop (enat 0) (llist s) \<in> llist ` set ss
-      \<and> remove_lqueue_step_w_details (lnth QDs j) ss (lnth QDs (Suc j))"
-      using zero_enat_def by auto
-    hence ?case
-      using j_ge by auto
-  }
-  moreover
-  {
-    assume "pick_lqueue_step_w_details (lnth QDs j) (lhd (llist s)) (ltl (llist s))
-      (lnth QDs (Suc j))"
-    hence "pick_lqueue_step_w_details (lnth QDs j) (lnth (llist s) 0)
-      (ldrop (enat (Suc 0)) (llist s)) (lnth QDs (Suc j))"
-      by (smt (verit) the_enat_0 ldrop_0 lhd_ldrop pick_lqueue_step_w_details.cases
-          pick_lqueue_step_w_detailsI zero_enat_def zero_lt)
-    hence ?case
-      using j_ge by auto
-  }
-  ultimately show ?case
-    using rem_or_pick by blast
+  have es_in': "LCons (lnth es 0) (ldrop (Suc 0) es) \<in># llists (fst (lnth QDs i))"
+    using es_in by (metis zero_lt ldrop_0 ldrop_enat ldropn_Suc_conv_ldropn zero_enat_def)
+  show ?case
+    using fair[OF chain inf es_in']
+    by (metis dual_order.refl ldrop_enat ldropn_Suc_conv_ldropn zero_lt)
 next
   case (Suc k)
   note ih = this(1) and sk_lt = this(2)
 
-  have k_lt: "enat k < llength (llist s)"
+  have k_lt: "enat k < llength es"
     using sk_lt Suc_ile_eq order_less_imp_le by blast
 
   obtain j :: nat where
     j_ge: "j \<ge> i" and
-    rem_or_pick_step: "(\<exists>k' \<le> k. \<exists>ss. ldrop (enat k') (llist s) \<in> set (map llist ss) \<and>
-        remove_lqueue_step_w_details (lnth QDs j) ss (lnth QDs (Suc j)))
-      \<or> pick_lqueue_step_w_details (lnth QDs j) (lnth (llist s) k) (ldrop (enat (Suc k)) (llist s))
+    rem_or_pick_step: "(\<exists>k' \<le> k. \<exists>ess. ldrop (enat k') es \<in> set ess
+        \<and> remove_lqueue_step_w_details (lnth QDs j) ess (lnth QDs (Suc j)))
+      \<or> pick_lqueue_step_w_details (lnth QDs j) (lnth es k) (ldrop (enat (Suc k)) es)
         (lnth QDs (Suc j))"
     using ih[OF k_lt] by blast
 
   {
-    assume "\<exists>k' \<le> k. \<exists>ss. ldrop (enat k') (llist s) \<in> set (map llist ss) \<and>
-      remove_lqueue_step_w_details (lnth QDs j) ss (lnth QDs (Suc j))"
+    assume "\<exists>k' \<le> k. \<exists>ess. ldrop (enat k') es \<in> set ess
+      \<and> remove_lqueue_step_w_details (lnth QDs j) ess (lnth QDs (Suc j))"
     hence ?case
       using j_ge le_SucI by blast
   }
   moreover
   {
-    assume pick_step: "pick_lqueue_step_w_details (lnth QDs j) (lnth (llist s) k)
-      (ldrop (enat (Suc k)) (llist s)) (lnth QDs (Suc j))"
+    assume "pick_lqueue_step_w_details (lnth QDs j) (lnth es k) (ldrop (enat (Suc k)) es)
+      (lnth QDs (Suc j))"
+    hence cons_in: "LCons (lnth es (Suc k)) (ldrop (enat (Suc (Suc k))) es)
+      \<in># llists (fst (lnth QDs (Suc j)))"
+      unfolding pick_lqueue_step_w_details.simps using sk_lt
+      by (metis fst_conv ldrop_enat ldropn_Suc_conv_ldropn union_mset_add_mset_right
+          union_single_eq_member)
 
-    obtain s' :: 's where
-      s_at_k: "lnth (llist s) k = e" and
-      s_from_sk: "ldrop (enat (Suc k)) (llist s) = es" ans
-
-      s'_in: "s' \<in># streams (fst (lnth QDs j))" and
-      s'_nnil: "llist s' \<noteq> LNil"
-      using pick_step unfolding pick_lqueue_step_w_details.simps by (metis fst_conv)
-    obtain s'' :: 's where
-      s'': "llist s'' = ltl (llist s')"
-      using exists_stream by blast
-
-    obtain j' where
-      j'_ge: "j' \<ge> j" and
-      rem_or_pick: "(\<exists>ss. s' \<in> set ss \<and> remove_lqueue_step_w_details (lnth QDs j') ss
-          (lnth QDs (Suc j')))
-        \<or> pick_lqueue_step_w_details (lnth QDs j') (lhd (llist s')) (ltl (llist s'))
-          (lnth QDs (Suc j'))"
-      using fair[OF chain inf s'_in s'_nnil s''] by blast
-
-    {
-      assume rem_step': "\<exists>ss. s' \<in> set ss \<and> remove_lqueue_step_w_details (lnth QDs j') ss
-        (lnth QDs (Suc j'))"
-
-      have "\<exists>k' \<le> Suc k. \<exists>ss.
-        ldrop (enat k') (llist s) \<in> set (map llist ss) \<and>
-        remove_lqueue_step_w_details (lnth QDs j') ss (lnth QDs (Suc j'))"
-        apply (rule exI[of _ 0])
-        sorry
-      hence ?case
-        using j'_ge j_ge order.trans by blast
-    }
-    moreover
-    {
-      assume pick_step': "pick_lqueue_step_w_details (lnth QDs j') (lhd (llist s')) (ltl (llist s'))
-        (lnth QDs (Suc j'))"
-      have "\<exists>j \<ge> i. pick_lqueue_step_w_details (lnth QDs j) (lnth (llist s) (Suc k))
-        (ldrop (enat (Suc (Suc k))) (llist s)) (lnth QDs (Suc j))"
-        sorry
-      hence ?case
-        sorry
-    }
-    ultimately have ?case
-      using rem_or_pick by blast
+    have ?case
+      using fair[OF chain inf cons_in] j_ge
+      by (smt (z3) dual_order.trans ldrop_enat ldropn_Suc_conv_ldropn le_Suc_eq sk_lt)
   }
   ultimately show ?case
     using rem_or_pick_step by blast
+qed
+
+end
+
+
+subsection \<open>Instantiation with FIFO Queue\<close>
+
+text \<open>As a proof of concept, we show that a FIFO queue can serve as a fair
+prover lazy list queue.\<close>
+
+(* TODO: Separate between nils and cons, use a counter to represent nils, use a pair to represent
+cons. *)
+
+locale fifo_prover_lazy_list_queue
+begin
+
+fun pick_elem :: "'e llist list \<Rightarrow> 'e \<times> 'e llist list" where
+  "pick_elem [] = undefined"
+| "pick_elem (LNil # ess) =
+   (let (e, ess') = pick_elem ess in
+      (e, ess' @ [LNil]))"
+| "pick_elem (LCons e es # ess) = (e, ess @ [es])"
+
+sublocale prover_lazy_list_queue "[]" "\<lambda>es ess. ess @ [es]" remove1 pick_elem mset
+proof
+  fix Q :: "'e llist list"
+  assume ex_cons: "\<exists>es \<in># mset Q. es \<noteq> LNil"
+  show "\<exists>e es. LCons e es \<in># mset Q \<and> fst (pick_elem Q) = e
+      \<and> mset (snd (pick_elem Q)) = mset Q - {#LCons e es#} + {#es#}"
+    using ex_cons
+  proof (induct Q rule: pick_elem.induct)
+    case 1
+    note ex_cons = this(1)
+    have False
+      using ex_cons by simp
+    thus ?case
+      by blast
+  next
+    case (2 ess)
+    note ih = this(1) and ex_cons = this(2)
+
+    obtain e :: 'e and es :: "'e llist" where
+      "LCons e es \<in># mset ess" and
+      "fst (pick_elem ess) = e" and
+      "mset (snd (pick_elem ess)) = mset ess - {#LCons e es#} + {#es#}"
+      using ih ex_cons by auto
+    thus ?case
+      by (auto simp: case_prod_beta)
+  next
+    case (3 e es ess)
+    show ?case
+      using add_mset_diff_bothsides by auto
+  qed
+qed simp+
+
+sublocale fair_prover_lazy_list_queue "[]" "\<lambda>es ess. ess @ [es]" remove1 pick_elem mset
+proof
+  fix
+    QDs :: "('e llist list \<times> 'e set) llist" and
+    i :: nat and
+    e :: 'e and
+    es :: "'e llist"
+  assume
+    chain: "chain lqueue_step QDs" and
+    inf_pick: "infinitely_often pick_lqueue_step QDs" and
+    cons_in: "LCons e es \<in># mset (fst (lnth QDs i))"
+
+  have len: "llength QDs = \<infinity>"
+    using inf_pick unfolding infinitely_often_alt_def
+    by (metis Suc_ile_eq dual_order.strict_implies_order enat.exhaust enat_ord_simps(2)
+        verit_comp_simplify1(3))
+
+  {
+    assume not_rem_step: "\<not> (\<exists>j \<ge> i. \<exists>ess. LCons e es \<in> set ess
+      \<and> remove_lqueue_step_w_details (lnth QDs j) ess (lnth QDs (Suc j)))"
+
+    obtain k :: nat where
+      k_lt: "k < length (fst (lnth QDs i))" and
+      at_k: "fst (lnth QDs i) ! k = LCons e es"
+      using cons_in by (metis in_set_conv_nth set_mset_mset)
+
+    have "\<forall>k' \<le> k. \<exists>i' \<ge> i. LCons e es \<in># mset (take (Suc k') (fst (lnth QDs i')))"
+    proof -
+      have "\<exists>i' \<ge> i. LCons e es \<in># mset (take (k + 1 - l) (fst (lnth QDs i')))"
+        if l_le: "l \<le> k" for l
+        using l_le
+      proof (induct l)
+        case 0
+        show ?case
+        proof (rule exI[of _ i]; simp)
+          show "LCons e es \<in> set (take (Suc k) (fst (lnth QDs i)))"
+            by (simp add: at_k k_lt take_Suc_conv_app_nth)
+        qed
+      next
+        case (Suc l)
+        note ih = this(1) and sl_le = this(2)
+
+        have l_le_k: "l \<le> k"
+          using sl_le by linarith
+        note ih = ih[OF l_le_k]
+
+        obtain i' :: nat where
+          i'_ge: "i' \<ge> i" and
+          cons_at_i': "LCons e es \<in># mset (take (k + 1 - l) (fst (lnth QDs i')))"
+          using ih by blast
+        then obtain j0 :: nat where
+          "j0 \<ge> i'" and
+          "pick_lqueue_step (lnth QDs j0) (lnth QDs (Suc j0))"
+          using inf_pick unfolding infinitely_often_alt_def by auto
+        then obtain j :: nat where
+          j_ge: "j \<ge> i'" and
+          pick_step: "pick_lqueue_step (lnth QDs j) (lnth QDs (Suc j))" and
+          pick_step_min:
+          "\<forall>j'. j' \<ge> i' \<longrightarrow> j' < j \<longrightarrow> \<not> pick_lqueue_step (lnth QDs j') (lnth QDs (Suc j'))"
+          using wfP_exists_minimal[OF wfP_less, of
+              "\<lambda>j. j \<ge> i' \<and> pick_lqueue_step (lnth QDs j) (lnth QDs (Suc j))" j0 "\<lambda>j. j"]
+          by blast
+
+        have cons_at_le_j: "LCons e es \<in># mset (take (k + 1 - l) (fst (lnth QDs j')))"
+          if j'_ge: "j' \<ge> i'" and j'_le: "j' \<le> j" for j'
+        proof -
+          have "LCons e es \<in># mset (take (k + 1 - l) (fst (lnth QDs (i' + m))))"
+            if i'm_le: "i' + m \<le> j" for m
+            using i'm_le
+          proof (induct m)
+            case 0
+            then show ?case
+              using cons_at_i' by fastforce
+          next
+            case (Suc m)
+            note ih = this(1) and i'sm_le = this(2)
+
+            have i'm_lt: "i' + m < j"
+              using i'sm_le by linarith
+            have i'm_le: "i' + m \<le> j"
+              using i'sm_le by linarith
+            note ih = ih[OF i'm_le]
+
+            have step: "lqueue_step (lnth QDs (i' + m)) (lnth QDs (i' + Suc m))"
+              by (simp add: chain chain_lnth_rel len)
+
+            show ?case
+              using step
+            proof cases
+              case (lqueue_step_fold_add_llistI Q D ess)
+              note defs = this
+              show ?thesis
+                using ih unfolding defs
+                by (auto intro: in_set_take_imp_in_set_take_fold_append_single)
+            next
+              case (lqueue_step_fold_remove_llistI Q D ess)
+              note defs = this
+              have "remove_lqueue_step_w_details (lnth QDs (i' + m)) ess (lnth QDs (i' + Suc m))"
+                unfolding defs by (rule remove_lqueue_step_w_detailsI)
+              hence "LCons e es \<notin> set ess"
+                using not_rem_step i'_ge by force
+              thus ?thesis
+                using ih unfolding defs
+                by (auto intro: notin_set_and_in_set_take_imp_in_set_take_fold_remove1)
+            next
+              case (lqueue_step_pick_elemI Q D)
+              note defs = this(1,2) and rest = this(3)
+
+              have "pick_lqueue_step (lnth QDs (i' + m)) (lnth QDs (i' + Suc m))"
+              proof -
+                have "\<exists>e es. pick_lqueue_step_w_details (lnth QDs (i' + m)) e es
+                  (lnth QDs (i' + Suc m))"
+                  unfolding defs using pick_lqueue_step_w_detailsI
+                  by (metis add_Suc_right llists_pick_elem lqueue_step_pick_elemI(2) rest)
+                thus ?thesis
+                  using pick_lqueue_stepI by fast
+              qed
+
+              thm pick_step_min[rule_format, OF le_add1]
+
+              moreover have "\<not> pick_lqueue_step (lnth QDs (i' + m)) (lnth QDs (i' + Suc m))"
+                using pick_step_min[rule_format, OF le_add1 i'm_lt] by simp
+              ultimately show ?thesis
+                by blast
+            qed
+          qed
+          thus ?thesis
+            by (metis j'_ge j'_le nat_le_iff_add)
+        qed
+
+        show ?case
+        proof (rule exI[of _ "Suc j"], intro conjI)
+          show "i \<le> Suc j"
+            using i'_ge j_ge by linarith
+        next
+          obtain Q :: "'e llist list" and D :: "'e set" and e' :: 'e and es' :: "'e llist" where
+            at_j: "lnth QDs j = (Q, D)" and
+            at_sj: "lnth QDs (Suc j) = (snd (pick_elem Q), D \<union> {e'})" and
+            ees'_in: "LCons e' es' \<in># mset Q" and
+            fst: "fst (pick_elem Q) = e'" and
+            snd: "mset (snd (pick_elem Q)) = mset Q - {#LCons e' es'#} + {#es'#}"
+            using pick_step unfolding pick_lqueue_step.simps pick_lqueue_step_w_details.simps
+            by blast
+
+          have cons_at_j: "LCons e es \<in># mset (take (k + 1 - l) (fst (lnth QDs j)))"
+            using cons_at_le_j[of j] j_ge by blast
+
+          show "LCons e es \<in># mset (take (k + 1 - Suc l) (fst (lnth QDs (Suc j))))"
+            using cons_at_j unfolding at_j at_sj
+(*
+characterize "snd (pick_elem Q)" using an inductive lemma
+*)
+            sorry
+        qed
+      qed
+      thus ?thesis
+        by (metis Suc_eq_plus1 add_right_mono diff_Suc_Suc diff_diff_cancel diff_le_self)
+    qed
+    then obtain i' :: nat where
+      i'_ge: "i' \<ge> i" and
+      cons_at_i': "LCons e es \<in># mset (take 1 (fst (lnth QDs i')))"
+      by auto
+    then obtain j0 :: nat where
+      "j0 \<ge> i'" and
+      "pick_lqueue_step (lnth QDs j0) (lnth QDs (Suc j0))"
+      using inf_pick unfolding infinitely_often_alt_def by auto
+    then obtain j :: nat where
+      j_ge: "j \<ge> i'" and
+      pick_step: "pick_lqueue_step (lnth QDs j) (lnth QDs (Suc j))" and
+      pick_step_min:
+        "\<forall>j'. j' \<ge> i' \<longrightarrow> j' < j \<longrightarrow> \<not> pick_lqueue_step (lnth QDs j') (lnth QDs (Suc j'))"
+      using wfP_exists_minimal[OF wfP_less, of
+         "\<lambda>j. j \<ge> i' \<and> pick_lqueue_step (lnth QDs j) (lnth QDs (Suc j))" j0 "\<lambda>j. j"]
+      by blast
+    hence pick_step_det: "\<exists>e es. pick_lqueue_step_w_details (lnth QDs j) e es (lnth QDs (Suc j))"
+      unfolding pick_lqueue_step.simps by simp
+    have "pick_lqueue_step_w_details (lnth QDs j) e es (lnth QDs (Suc j))"
+    proof -
+      have cons_at_j: "LCons e es \<in># mset (take 1 (fst (lnth QDs j)))"
+      proof -
+        have "LCons e es \<in># mset (take 1 (fst (lnth QDs (i' + l))))" if i'l_le: "i' + l \<le> j" for l
+          using i'l_le
+        proof (induct l)
+          case (Suc l)
+          note ih = this(1) and i'sl_le = this(2)
+
+          have i'l_lt: "i' + l < j"
+            using i'sl_le by linarith
+          have i'l_le: "i' + l \<le> j"
+            using i'sl_le by linarith
+          note ih = ih[OF i'l_le]
+
+          have step: "lqueue_step (lnth QDs (i' + l)) (lnth QDs (i' + Suc l))"
+            by (simp add: chain chain_lnth_rel len)
+
+          show ?case
+            using step
+          proof cases
+            case (lqueue_step_fold_add_llistI Q D ess)
+            note defs = this
+
+            have len_q: "length Q \<ge> 1"
+              using ih by (metis Suc_eq_plus1 add.commute empty_iff le_add1 length_0_conv list.set(1)
+                  list_decode.cases local.lqueue_step_fold_add_llistI(1) prod.sel(1) set_mset_mset
+                  take.simps(1))
+
+            have take: "take (Suc 0) (fold (\<lambda>es ess. ess @ [es]) ess Q) = take (Suc 0) Q"
+              using len_q
+            proof (induct ess arbitrary: Q)
+              case (Cons es ess)
+              note ih = this(1) and len_q = this(2)
+              show ?case
+                using len_q by (simp add: ih)
+            qed auto
+
+            show ?thesis
+              unfolding defs using ih take
+              by simp (metis local.lqueue_step_fold_add_llistI(1) prod.sel(1))
+          next
+            case (lqueue_step_fold_remove_llistI Q D ess)
+            note defs = this
+
+            have "remove_lqueue_step_w_details (lnth QDs (i' + l)) ess (lnth QDs (i' + Suc l))"
+              unfolding defs by (rule remove_lqueue_step_w_detailsI)
+            moreover have "\<not> (\<exists>ess. LCons e es \<in> set ess
+              \<and> remove_lqueue_step_w_details (lnth QDs (i' + l)) ess (lnth QDs (i' + Suc l)))"
+              using not_rem_step add_Suc_right i'_ge trans_le_add1 by presburger
+            ultimately have ees_ni: "LCons e es \<notin> set ess"
+              by blast
+
+            obtain Q' :: "'e llist list" where
+              q: "Q = LCons e es # Q'"
+              using ih by (metis One_nat_def fst_eqD in_set_member in_set_takeD length_pos_if_in_set
+                  list.exhaust_sel lqueue_step_fold_remove_llistI(1) member_rec nth_Cons_0
+                  set_mset_mset take0 take_Suc_conv_app_nth)
+
+            have take_1: "take 1 (fold remove1 ess Q) = take 1 Q"
+              unfolding q using ees_ni
+            proof (induct ess arbitrary: Q')
+              case (Cons es' ess')
+              note ih = this(1) and ees_ni = this(2)
+
+              have ees_ni': "LCons e es \<notin> set ess'"
+                using ees_ni by simp
+              note ih = ih[OF ees_ni']
+
+              have "es' \<noteq> LCons e es"
+                using ees_ni by auto
+              thus ?case
+                using ih by simp
+            qed auto
+
+            show ?thesis
+              unfolding defs using ih take_1
+              by simp (metis lqueue_step_fold_remove_llistI(1) prod.sel(1))
+          next
+            case (lqueue_step_pick_elemI Q D)
+            note defs = this(1,2) and rest = this(3)
+
+            have "pick_lqueue_step (lnth QDs (i' + l)) (lnth QDs (Suc (i' + l)))"
+            proof -
+              have "\<exists>e es. pick_lqueue_step_w_details (lnth QDs (i' + l)) e es
+                (lnth QDs (Suc (i' + l)))"
+                unfolding defs using pick_lqueue_step_w_detailsI
+                by (metis add_Suc_right llists_pick_elem lqueue_step_pick_elemI(2) rest)
+              thus ?thesis
+                using pick_lqueue_stepI by fast
+            qed
+            moreover have "\<not> pick_lqueue_step (lnth QDs (i' + l)) (lnth QDs (Suc (i' + l)))"
+              using pick_step_min[rule_format, OF le_add1 i'l_lt] .
+            ultimately show ?thesis
+              by blast
+          qed
+        qed (use cons_at_i' in auto)
+        thus ?thesis
+          by (metis dual_order.refl j_ge nat_le_iff_add)
+      qed
+      hence cons_in_fst: "LCons e es \<in># mset (fst (lnth QDs j))"
+        using in_set_takeD by force
+
+      obtain Q' :: "'e llist list" where
+        fst_at_j: "fst (lnth QDs j) = LCons e es # Q'"
+        using cons_at_j by (metis (no_types, lifting) One_nat_def cons_in_fst empty_iff empty_set
+            fifo_prover_lazy_list_queue.pick_elem.elims length_pos_if_in_set nth_Cons_0
+            self_append_conv2 set_ConsD set_mset_mset take0 take_Suc_conv_app_nth)
+
+      have fst_pick: "fst (pick_elem (fst (lnth QDs j))) = e"
+        unfolding fst_at_j by simp
+      have snd_pick: "mset (snd (pick_elem (fst (lnth QDs j)))) =
+        mset (fst (lnth QDs j)) - {#LCons e es#} + {#es#}"
+        unfolding fst_at_j by simp
+
+      show ?thesis
+        using cons_in_fst fst_pick snd_pick
+        by (smt (verit, ccfv_SIG) pick_step_det fst_conv pick_lqueue_step_w_details.simps)
+    qed
+    hence "\<exists>j \<ge> i. pick_lqueue_step_w_details (lnth QDs j) e es (lnth QDs (Suc j))"
+      using i'_ge j_ge le_trans by blast
+  }
+  thus "\<exists>j \<ge> i.
+      (\<exists>ess. LCons e es \<in> set ess \<and> remove_lqueue_step_w_details (lnth QDs j) ess (lnth QDs (Suc j)))
+    \<or> pick_lqueue_step_w_details (lnth QDs j) e es (lnth QDs (Suc j))"
+    by blast
 qed
 
 end
